\begin{problem}{1}
Solve this problem with Induction \\
\subsection*{Basis Step}
\begin{align*}
{C(1)} &= \frac{1}{4} \cdot ({(1)^4} + 2 \cdot {(1)^3} + {(1)^2}) = 1\\
{1^3} &= 1\surd
\end{align*}
\subsection*{Inductive Step}
\begin{align*}
{1^3} + {2^3} + ... + {k^3} + {(k + 1)^3} &= \frac{1}{4}({(k + 1)^4} + 2{(k + 1)^3} + {(k + 1)^2})\\
\frac{1}{4}{\rm{(}}{{\rm{k}}^4}{\rm{  +  2}}{{\rm{k}}^3}{\rm{  +  }}{{\rm{k}}^2}{\rm{)  +  (k  +  1}}{{\rm{)}}^3} &= \frac{1}{4}({(k + 1)^4} + 2{(k + 1)^3} + {(k + 1)^2})\\
& = \frac{1}{4}({k^4} + 4{k^3} + 6{k^2} + 4k + 1 + 2{k^3} + 6{k^2} + 6k + 2 + {k^2} + 2k + 1)\\
& = \frac{1}{4}({k^4} + 2{k^3} + {k^2}) + \frac{1}{4}(4{k^3} + 6{k^2} + 6{k^2} + 4k + 6k + 2k + 1 + 2 + 1)\\
& = \frac{1}{4}({k^4} + 2{k^3} + {k^2}) + \frac{1}{4}(4{k^3} + 12{k^2} + 12k + 4)\\
& = \frac{1}{4}({k^4} + 2{k^3} + {k^2}) + {k^3} + 3{k^2} + 3k + 1\\
& = \frac{1}{4}({k^4} + 2{k^3} + {k^2}) + {(k + 1)^3}
\end{align*}
\hfill Q.E.D
\end{problem}
